@prefix def-dclg: <http://opendatacommunities.org/def/local-government/> .
@prefix owl:   <http://www.w3.org/2002/07/owl#> .
@prefix def-geom: <http://location.data.gov.uk/def/common/Geometry/> .
@prefix def-sp: <http://location.data.gov.uk/def/ef/SamplingPoint/> .
@prefix def-cc12: <http://environment.data.gov.uk/def/bwq-cc-2012/> .
@prefix def-bwp: <http://environment.data.gov.uk/def/bathing-water-profile/> .
@prefix xsd:   <http://www.w3.org/2001/XMLSchema#> .
@prefix skos:  <http://www.w3.org/2004/02/skos/core#> .
@prefix spatialrelations: <http://data.ordnancesurvey.co.uk/ontology/spatialrelations/> .
@prefix rdfs:  <http://www.w3.org/2000/01/rdf-schema#> .
@prefix def-bwq: <http://environment.data.gov.uk/def/bathing-water-quality/> .
@prefix geo:   <http://www.w3.org/2003/01/geo/wgs84_pos#> .
@prefix chterms: <http://business.data.gov.uk/companies/def/terms/> .
@prefix def-ddr: <http://environment.data.gov.uk/def/dedesignation-reason/> .
@prefix qb:    <http://purl.org/linked-data/cube#> .
@prefix dgu:   <http://reference.data.gov.uk/def/reference/> .
@prefix dct:   <http://purl.org/dc/terms/> .
@prefix reg:   <http://purl.org/linked-data/registry#> .
@prefix wqa-sp: <http://environment.data.gov.uk/water-quality/def/sampling-point/> .
@prefix def-incident-type: <http://environment.data.gov.uk/def/incident-type/> .
@prefix def-stp: <http://environment.data.gov.uk/def/bwq-stp/> .
@prefix admingeo: <http://data.ordnancesurvey.co.uk/ontology/admingeo/> .
@prefix foaf:  <http://xmlns.com/foaf/0.1/> .
@prefix void:  <http://rdfs.org/ns/void#> .
@prefix onsadmingeo: <http://statistics.data.gov.uk/def/administrative-geography/> .
@prefix org:   <http://www.w3.org/ns/org#> .
@prefix def-ver: <http://environment.data.gov.uk/def/version/> .
@prefix so-sp: <http://location.data.gov.uk/so/ef/SamplingPoint/bwsp.eaew/> .
@prefix def-zoi: <http://location.data.gov.uk/def/ef/ZoneOfInfluence/> .
@prefix id-bw: <http://environment.data.gov.uk/id/bathing-water/> .
@prefix intervals: <http://reference.data.gov.uk/def/intervals/> .
@prefix def-som: <http://environment.data.gov.uk/def/bwq-som/> .
@prefix rdf:   <http://www.w3.org/1999/02/22-rdf-syntax-ns#> .
@prefix def-feat: <http://location.data.gov.uk/def/ef/BathingWaterProfileFeature/> .
@prefix interval: <http://reference.data.gov.uk/def/intervals/> .
@prefix geometry: <http://data.ordnancesurvey.co.uk/ontology/geometry/> .
@prefix geowgs84: <http://www.w3.org/2003/01/geo/wgs84_pos#> .
@prefix time:  <http://www.w3.org/2006/time#> .
@prefix status: <http://reference.data.gov.uk/def/status/> .
@prefix def-bw: <http://environment.data.gov.uk/def/bathing-water/> .

def-ddr:PAAB-TI  a      skos:Concept , def-ddr:DedesignationReasonCode ;
        rdfs:comment    "Permanent advice against bathing is in place at this water. It is no longer designated as a bathing water under the Bathing Water Regulations 2013 because it is infeasible to meet the minimum, legally required bathing water quality standard at this location."@en ;
        rdfs:label      "Permanent advice against bathing, Technically infeasible"@en ;
        skos:broader    def-ddr:PAAB ;
        skos:inScheme   def-ddr:DedesignationReasonScheme ;
        skos:notation   "PAAB-TI" ;
        skos:prefLabel  "Permanent advice against bathing, Technically infeasible"@en .

def-ddr:PAAB-DEXP  a    skos:Concept , def-ddr:DedesignationReasonCode ;
        rdfs:comment    "Permanent advice against bathing is in place at this water.\nIt is no longer designated as a bathing water under the Bathing Water Regulations 2013 because the costs of meeting the minimum, legally required bathing water quality standard are disproportionately expensive."@en ;
        rdfs:label      "Permanent advice against bathing, Disproportionately expensive"@en ;
        skos:broader    def-ddr:PAAB ;
        skos:inScheme   def-ddr:DedesignationReasonScheme ;
        skos:notation   "PAAB-DEXP" ;
        skos:prefLabel  "Permanent advice against bathing, Disproportionately expensive"@en .

def-ddr:DedesignationReasonScheme
        a                   skos:ConceptScheme ;
        rdfs:label          "A SKOS ConceptScheme for bathing water dedesignation coded reasons."@en ;
        skos:hasTopConcept  def-ddr:PAAB , def-ddr:LOW , def-ddr:CBO .

def-ddr:PAAB-CP  a      skos:Concept , def-ddr:DedesignationReasonCode ;
        rdfs:comment    "Permanent advice against bathing is in place at this water. It is no longer designated as a bathing water under the Bathing Water Regulations 2013 because the water has been classified as poor for five consecutive years."@en ;
        rdfs:label      "Permanent advice against bathing, Classified poor"@en ;
        skos:broader    def-ddr:PAAB ;
        skos:inScheme   def-ddr:DedesignationReasonScheme ;
        skos:notation   "PAAB-CP" ;
        skos:prefLabel  "Permanent advice against bathing, Classified poor"@en .

def-ddr:dedesignationReasonText
        a             owl:DatatypeProperty ;
        rdfs:comment  "A property for associating a dedesignated bathing-water with a narrative reason for its dedesignation."@en ;
        rdfs:domain   def-bw:BathingWater ;
        rdfs:label    "dedesignationReasonText" ;
        rdfs:range    def-ddr:DedesignationReasonCode .

def-ddr:PAAB  a            def-ddr:DedesignationReasonCode , skos:Concept ;
        rdfs:label         "Permanent advice against bathing"@en ;
        skos:inScheme      def-ddr:DedesignationReasonScheme ;
        skos:narrower      def-ddr:PAAB-CP , def-ddr:PAAB-TI , def-ddr:PAAB-DEXP ;
        skos:notation      "PAAB" ;
        skos:prefLabel     "Permanent advice against bathing"@en ;
        skos:topConceptOf  def-ddr:DedesignationReasonScheme .

def-ddr:CBO  a             skos:Concept , def-ddr:DedesignationReasonCode ;
        rdfs:label         "De-listed access closed by private owner"@en ;
        skos:inScheme      def-ddr:DedesignationReasonScheme ;
        skos:notation      "CBO" ;
        skos:prefLabel     "De-listed access closed by private owner"@en ;
        skos:topConceptOf  def-ddr:DedesignationReasonScheme .

def-ddr:dedesignationReasonCode
        a             owl:ObjectProperty ;
        rdfs:comment  "A property for associating a dedesignated bathing-water with a coded reason for its dedesignation."@en ;
        rdfs:domain   def-bw:BathingWater ;
        rdfs:label    "dedesignationReasonCode" ;
        rdfs:range    def-ddr:DedesignationReasonCode .

def-ddr:DedesignationReasonCode
        a                owl:Class ;
        rdfs:comment     "A subclass of SKOS Concept for bathing water dedesignation coded reasons."@en ;
        rdfs:label       "DedesignationReasonCode" ;
        rdfs:subClassOf  skos:Concept .

def-ddr:LOW  a             skos:Concept , def-ddr:DedesignationReasonCode ;
        rdfs:label         "De-listed low usage for bathing"@en ;
        skos:inScheme      def-ddr:DedesignationReasonScheme ;
        skos:notation      "LOW" ;
        skos:prefLabel     "De-listed low usage for bathing"@en ;
        skos:topConceptOf  def-ddr:DedesignationReasonScheme .
